ok

SStructTT/Static/Renaming.lean
@@ -1,16 +1,197 @@
 import SStructTT.Static.Typed
 
 namespace Static
-variable {Srt : Type} [SStruct Srt]
+variable {Srt : Type} [inst : SStruct Srt]
 
+@[aesop safe (rule_sets := [rename]) [constructors]]
 inductive AgreeRen : (Var -> Var) -> Ctx Srt -> Ctx Srt -> Prop where
   | nil {ξ} :
     AgreeRen ξ  [] []
-  | cons Γ Γ' A s i ξ :
+  | cons {Γ Γ' A s i ξ} :
     Typed Γ A (.srt s i) ->
     AgreeRen ξ Γ Γ' ->
     AgreeRen (upren ξ) (A :: Γ) (A.[ren ξ] :: Γ')
-  | wk Γ Γ' A s i ξ :
+  | wk {Γ Γ' A s i ξ} :
     Typed Γ' A (.srt s i) ->
     AgreeRen ξ Γ Γ' ->
     AgreeRen (ξ !>> (.+1)) Γ (A :: Γ')
+
+@[aesop safe (rule_sets := [rename])]
+lemma AgreeRen.refl {Γ : Ctx Srt} : Wf Γ -> AgreeRen id Γ Γ := by
+  intro wf
+  induction wf
+  all_goals try trivial
+  case nil => constructor
+  case cons Γ A s i ty wf _ ih =>
+    have h := AgreeRen.cons ty ih
+    asimp at h
+    assumption
+
+lemma AgreeRen.has {Γ Γ' : Ctx Srt} {A x ξ} :
+    AgreeRen ξ Γ Γ' -> Has Γ x A -> Has Γ' (ξ x) A.[ren ξ] := by
+  intro agr
+  induction agr generalizing x A with
+  | nil => intro h; cases h
+  | @cons _ _ A _ _ ξ _ _ ih =>
+    intro h
+    cases h <;> asimp
+    case zero =>
+      have : A.[ren ξ >> shift 1] = A.[ren ξ].[shift 1] := by asimp
+      rw[this]; constructor
+    case succ A x hs =>
+      have : A.[ren ξ >> shift 1] = A.[ren ξ].[shift 1] := by asimp
+      rw[this]; constructor
+      apply ih; assumption
+  | @wk _ _ A _ _ ξ _ _ ih =>
+    intro h; asimp
+    have : A.[ren (ξ !>> .succ)] = A.[ren ξ].[shift 1] := by asimp; rfl
+    rw[this]; constructor
+    apply ih; assumption
+
+lemma AgreeRen.wf_nil {Γ' : Ctx Srt} {ξ} : AgreeRen ξ [] Γ' -> Wf Γ' := by
+  intro agr
+  cases agr with
+  | nil => constructor
+  | wk ty agr =>
+    constructor
+    . assumption
+    . apply ty.toWf
+
+lemma AgreeRen.wf_cons {Γ Γ' : Ctx Srt} {A ξ} :
+    AgreeRen ξ (A :: Γ) Γ' -> Wf Γ ->
+    (∀ Γ' ξ, AgreeRen ξ Γ Γ' → Wf Γ') ->
+    (∀ Γ' ξ, AgreeRen ξ Γ Γ' → ∃ s i, Typed Γ' A.[ren ξ] (.srt s i)) ->
+    Wf Γ' := by
+  intro agr
+  cases agr with
+  | cons ty agr =>
+    intro wf h1 h2
+    have ⟨s, i, ty⟩ := h2 _ _ agr
+    constructor
+    . assumption
+    . apply h1; assumption
+  | wk ty agr =>
+    intros
+    constructor
+    . assumption
+    . exact ty.toWf
+
+lemma Typed.renaming {Γ Γ' : Ctx Srt} {A m ξ} :
+    Typed Γ m A -> AgreeRen ξ Γ Γ' -> Typed Γ' m.[ren ξ] A.[ren ξ] := by
+  intro ty
+  induction ty
+  using @Typed.rec _ inst (motive_2 := fun Γ _ => ∀ Γ' ξ, AgreeRen ξ Γ Γ' -> Wf Γ')
+  generalizing Γ' ξ with
+  | srt _ wf ih =>
+    intro; asimp; constructor
+    apply ih; assumption
+  | var wf hs ih =>
+    intro; asimp; constructor
+    . apply ih; assumption
+    . apply AgreeRen.has <;> assumption
+  | pi _ _ tyA _ ihA ihB =>
+    intro agr; asimp; constructor
+    . apply ihA; assumption
+    . have := ihB (agr.cons tyA)
+      asimp at this; assumption
+  | lam _ _ tyA _ ihA ihm =>
+    intro agr; asimp; constructor
+    . apply ihA; assumption
+    . have := ihm (agr.cons tyA)
+      asimp at this; assumption
+  | app tym tyn ihm ihn =>
+    intro agr; asimp
+    replace tym := ihm agr; asimp at tym
+    replace tyn := ihn agr; asimp at tyn
+    have ty := Typed.app tym tyn; asimp at ty
+    assumption
+  | sig _ _ tyA tyB ihA ihB =>
+    intro agr; asimp; constructor
+    . apply ihA; assumption
+    . have := ihB (agr.cons tyA)
+      asimp at this; assumption
+  | pair _ _ _ ihT ihm ihn =>
+    intro agr; asimp; constructor
+    . apply ihT; assumption
+    . apply ihm; assumption
+    . have := ihn agr
+      asimp at this; asimp; assumption
+  | @proj Γ A B C m n r s sC iC tyC tym tyn ihC ihm ihn =>
+    intro agr; asimp
+    cases tyC.toWf; case cons tyS =>
+    cases tyn.toWf; case cons wf _ =>
+    cases wf; case cons =>
+    replace ihC := ihC (agr.cons tyS)
+    replace ihm := ihm agr
+    have agr' : AgreeRen (upren (upren ξ)) (B :: A :: Γ)
+      (B.[ren (upren ξ)] :: A.[ren ξ] :: Γ') := by
+      aesop (rule_sets := [rename])
+    replace ihn := ihn agr'
+    asimp at ihC
+    asimp at ihm
+    have : C.[.pair (.var 1) (.var 0) r s .: shift 2].[ren (upren $ upren ξ)]
+         = C.[up (ren ξ)].[.pair (.var 1) (.var 0) r s .: shift 2] := by
+      asimp; rfl
+    rw[this] at ihn
+    rw[SubstLemmas.upren_up] at ihn
+    replace := Typed.proj ihC ihm ihn
+    asimp at this
+    assumption
+  | bool _ ih =>
+    intro; asimp; constructor;
+    apply ih; assumption
+  | tt _ ih =>
+    intro; asimp; constructor;
+    apply ih; assumption
+  | ff _ ih =>
+    intro; asimp; constructor;
+    apply ih; assumption
+  | @ite _ A _ _ _ _ _ tyA _ _ _ ihA ihm ihn1 ihn2 =>
+    intro agr; asimp
+    cases tyA.toWf; case cons tyb =>
+    replace ihA := ihA (agr.cons tyb); asimp at ihA
+    replace ihm := ihm agr; asimp at ihm
+    have e1 : A.[.tt .: ren ξ] = A.[up (ren ξ)].[.tt/] := by asimp
+    have e2 : A.[.ff .: ren ξ] = A.[up (ren ξ)].[.ff/] := by asimp
+    replace ihn1 := ihn1 agr; asimp at ihn1; rw[e1] at ihn1
+    replace ihn2 := ihn2 agr; asimp at ihn2; rw[e2] at ihn2
+    have := Typed.ite ihA ihm ihn1 ihn2
+    asimp at this; assumption
+  | id tyA tym tyn ihA ihm ihn =>
+    intro; asimp; constructor
+    . apply ihA; assumption
+    . apply ihm; assumption
+    . apply ihn; assumption
+  | rfl _ ih =>
+    intro; asimp; constructor
+    apply ih; assumption
+  | @rw _ A B _ _ a b _ _ tyB tym tyn ihB ihm ihn =>
+    intro agr; asimp
+    cases tyB.toWf; case cons wf tyI =>
+    cases wf; case cons tyA =>
+    replace ihB := ihB ((agr.cons tyA).cons tyI); asimp at ihB
+    replace ihm := ihm agr; asimp at ihm
+    replace ihn := ihn agr; asimp at ihn
+    simp[<-SubstLemmas.subst_comp] at ihB
+    have : B.[a.[ren ξ].rfl .: a.[ren ξ] .: ren ξ]
+         = B.[ids 0 .: ids 1 .: ren ξ >> shift 1 >> shift 1]
+            .[.rfl a.[ren ξ],a.[ren ξ]/] := by asimp
+    rw[this] at ihm
+    have := Typed.rw ihB ihm ihn
+    asimp at this; assumption
+  | conv eq tym tyB ihm ihB =>
+    intro agr
+    replace ihB := ihB agr; asimp at ihB
+    replace ihm := ihm agr
+    apply Typed.conv
+    . apply Conv.subst _ eq
+    . assumption
+    . assumption
+  | nil Γ' ξ agr => exact agr.wf_nil
+  | @cons _ _ s i _ _ ih _ _ _ agr =>
+    apply agr.wf_cons
+    . assumption
+    . assumption
+    . intros
+      exists s, i
+      apply ih; assumption
