SStructTT/Attr/Register.lean
@@ -6,3 +6,4 @@ register_simp_attr asimp
 
 -- Rule sets for Aesop solver.
 declare_aesop_rule_sets [red, conv, pstep] (default := false)
+declare_aesop_rule_sets [rename, subst] (default := false)
